Loom/PredTrans.lean
@@ -1,0 +1,76 @@
+import Loom.LatticeExt
+import Loom.Post
+
+open Lean.Order
+
+universe u v w x
+
+/-!
+# Exception Continuation Monad
+
+The continuation monad for weakest precondition transformers.
+-/
+
+def PredTrans (t : Type u) (e : Type v) (α : Type w) := (α → t) → e → t
+
+instance [PartialOrder t] : PartialOrder (PredTrans t e α) :=
+  inferInstanceAs (PartialOrder ((α → t) → e → t))
+
+instance [CCPO t] : CCPO (PredTrans t e α) :=
+  inferInstanceAs (CCPO ((α → t) → e → t))
+
+instance instMonadCont (t : Type u) (e : Type v) : Monad (PredTrans t e) where
+  pure x := fun post _epost => post x
+  bind x f := fun post epost => x (f · post epost) epost
+
+instance instLawfulMonadCont (t : Type u) (e : Type v) : LawfulMonad (PredTrans t e) where
+  map_const := rfl
+  id_map _ := rfl
+  seqLeft_eq _ _ := rfl
+  seqRight_eq _ _ := rfl
+  pure_seq _ _ := rfl
+  bind_pure_comp _ _ := rfl
+  bind_map _ _ := rfl
+  pure_bind _ _ := rfl
+  bind_assoc _ _ _ := rfl
+
+def PredTrans.monotone [PartialOrder l] [PartialOrder e] (pt : PredTrans l e α) :=
+  ∀ post post' epost epost', post ⊑ post' → epost ⊑ epost' → pt post epost ⊑ pt post' epost'
+
+-- instance monadExceptOfPredTrans (t : Type u) (ε : Type v) :
+--     MonadExceptOf ε (PredTrans t ((ε → t) × e)) where
+--   throw e := fun _post epost => epost.1 e
+--   tryCatch x handle := fun post epost => x post ((handle · post epost), epost.2)
+
+@[simp] theorem PredTrans.apply_map {l : Type u} {e : Type v} {α : Type w} [PartialOrder l]
+    (trans : PredTrans l e α) (f : α → β) (post : β → l) :
+  (f <$> trans) post = trans (post ∘ f) := rfl
+
+@[simp]
+abbrev EPost.cons.pushExcept {α : Type u} {ε : Type v} {l : Type w} {e : Type z}
+    (post : α → l) (epost : EPost.cons (ε → l) e) : Except ε α → l :=
+  fun
+  | .ok a => post a
+  | .error e => epost.head e
+
+/--
+Adds the ability to make assertions about exceptions of type `ε` to a predicate transformer with
+postcondition on exceptions of type `es`, resulting in postcondition on exceptions of type
+`(ε → l) :: es`.
+-/
+def PredTrans.pushExcept {α : Type u} {ε : Type v} {l : Type w} {e : Type z}
+    (x : PredTrans l e (Except ε α)) : PredTrans l (EPost.cons (ε → l) e) α :=
+  fun post epost => x (epost.pushExcept post) epost.tail
+
+/--
+Adds the ability to make assertions about a state of type `σ` to a predicate transformer with
+postcondition shape `es`, resulting in a transformer over `σ → l`.
+-/
+def pushArg {σ : Type u} {l : Type v} {e : Type w} {α : Type z}
+    (x : σ → PredTrans l e (α × σ)) : PredTrans (σ → l) e α :=
+  fun post epost s => x s (fun (a, s) => post a s) epost
+
+@[simp, grind =]
+theorem apply_pushArg {σ : Type u} {l : Type v} {e : Type w} {α : Type z}
+    (x : σ → PredTrans l e (α × σ)) (post : α → σ → l) (epost : e) (s : σ) :
+  (pushArg x) post epost s = x s (fun (a, s) => post a s) epost := rfl
